floyd/forward.v
@@ -1715,7 +1715,7 @@ intros; subst; auto.
 Qed.
 
 Lemma quick_derives_right:
-  forall P Q : mpred,
+  forall P Q : environ -> mpred,
    TT |-- Q -> P |-- Q.
 Proof.
 intros. eapply derives_trans; try eassumption; auto.
